Add Kappa based sequential semantics (#355)
* Add Kappa based sequential semantics

There are existing arrow sequential semantics, but this adds list based
(not single time step) kappa semantics, and shows they are at least
equivalent on the counter example.

There is an inefficiency in simulation of `Letrec`, I think this will
crop up with `loopBit` too. There may be a performant simple way to
express the evaluation I may have missed. Writing a more complex
performant version I will leave till later.

* Add 'SignalingCounter' to help explore sequential semantic proofs

arrow-examples/ArrowExamplesSV.hs
@@ -23,6 +23,7 @@ import Mux2_1
 import SyntaxExamples
 import UnsignedAdder
 import Counter
+import SignalingCounter
 import Fir
 import ArrowAdderTutorial
 
@@ -44,5 +45,7 @@ main = do
   writeTestBench growth_tree_8_tb
   writeSystemVerilog counter_3_netlist
   writeTestBench counter_3_tb
+  writeSystemVerilog signaling_counter_netlist
+  writeTestBench signaling_counter_tb
   writeSystemVerilog fir_netlist
   writeTestBench fir_tb
