silveroak-opentitan/aes/Arrow/pkg.v
@@ -22,28 +22,6 @@ Import VectorNotations.
 Import KappaNotation.
 Open Scope kind_scope.
 
-Notation "|^ x" :=
-  (App (CallModule (foldr1 <[\a b => xor a b]>)) x)
-  (in custom expr at level 5, no associativity) : kappa_scope.
-Notation "x && y" :=
-  (App (App (Primitive (P2 And)) x) y)
-  (in custom expr at level 6, left associativity) : kappa_scope.
-Notation "x || y" :=
-  (App (App (Primitive (P2 And)) x) y)
-  (in custom expr at level 6, left associativity) : kappa_scope.
-Notation "x & y" :=
-  (App (App (CallModule (bitwise <[and]>)) x) y)
-  (in custom expr at level 6, left associativity) : kappa_scope.
-Notation "x ^ y" :=
-  (App (App (CallModule (bitwise <[xor]>)) x) y)
-    (in custom expr at level 6, left associativity) : kappa_scope.
-Notation "'if' i 'then' t 'else' e" :=
-  (App (App (App (CallModule mux_item) i) t) e)
-  (in custom expr at level 5, left associativity) : kappa_scope.
-Notation "x == y" :=
-  (App (App (CallModule equality) x) y)
-  (in custom expr at level 6, left associativity) : kappa_scope.
-
 Inductive SboxImpl :=
 | SboxLut
 | SboxCanright
